src/test/isabelle/All_Tests.thy
@@ -1,38 +1,5 @@
 theory All_Tests
-  imports 
-    (* Tests *)
-    Test_Misc Test_Tactics Test_Encoding Test_QRHL_Core
-
-    (* Examples *)
-    "QRHL-Examples.Example" "QRHL-Examples.Teleport_Terse" "QRHL-Examples.Teleport"
-    "QRHL-Examples.Chsh" "QRHL-Examples.PrgEnc" "QRHL-Examples.Code_Example"
-    "QRHL-Examples.EPR" "QRHL-Examples.RandomOracle"
+  imports All_Unit_Tests All_Example_Thys
 begin
-
-ML \<open>
-
-val has_missing = Unsynchronized.ref false
-
-val tests =
-  \<^theory> |> Resources.master_directory |> File.read_dir
-  |> map_filter (fn f => 
-      if String.isSuffix ".thy" f andalso f <> "All_Tests.thy" andalso f <> "UnitTest.thy"
-      then SOME (substring (f, 0, String.size f - 4)) else NONE)
-
-val examples = \<^theory> |> Resources.master_directory |> (fn p => Path.append p (Path.explode "../../../examples")) |> File.read_dir
-  |> map_filter (fn f => if String.isSuffix ".thy" f andalso f <> "TestEx.thy"
-      then SOME (substring (f, 0, String.size f - 4)) else NONE)
-
-val theories = \<^theory> |> Context.parents_of |> map Context.theory_name
-
-val _ = tests |> map (fn f =>
-  if member op= theories f then () else (warning ("Add "^f^" to the imports"); has_missing := true))
-
-val _ = examples |> map (fn f =>
-  if member op= theories f then () else (warning ("Add \"QRHL-Examples."^f^"\" to the imports"); has_missing := true))
-
-val _ = if !has_missing then error "Please fix imports" else ()
-
-\<close>
 
 end
