src/test/isabelle/All_Unit_Tests.thy
@@ -1,0 +1,27 @@
+theory All_Unit_Tests
+  imports 
+    (* Tests *)
+    Test_Misc Test_Tactics Test_Encoding Test_QRHL_Core
+begin
+
+ML \<open>
+
+val has_missing = Unsynchronized.ref false
+
+val tests =
+  \<^theory> |> Resources.master_directory |> File.read_dir
+  |> map_filter (fn f => 
+      if String.isSuffix ".thy" f andalso f <> "All_Tests.thy" andalso f <> "UnitTest.thy" 
+        andalso f <> "All_Unit_Tests.thy" andalso f <> "All_Example_Thys.thy"
+      then SOME (substring (f, 0, String.size f - 4)) else NONE)
+
+val theories = \<^theory> |> Context.parents_of |> map Context.theory_name
+
+val _ = tests |> map (fn f =>
+  if member op= theories f then () else (warning ("Add "^f^" to the imports"); has_missing := true))
+
+val _ = if !has_missing then error "Please fix imports" else ()
+
+\<close>
+
+end
